Better LZ77 implementation.

code/c/Yazi_Misc.h
@@ -1,10 +1,20 @@
-#ifndef __Yazi_Allocator_H
-#define __Yazi_Allocator_H
+#ifndef __Yazi_Misc_H
+#define __Yazi_Misc_H
 
 #define KRML_HOST_MALLOC(size) (strm->zalloc(strm->opaque, 1, size))
 #define KRML_HOST_FREE(address) (strm->zfree(strm->opaque, address))
 
 typedef void *(*alloc_func) (void *opaque, unsigned int items, unsigned int size);
 typedef void (*free_func)  (void *opaque, void *address);
+
+static inline unsigned char is_little_endian(void)
+{
+  union {
+    unsigned int v;
+    unsigned char b;
+  } u;
+  u.v = 1;
+  return u.b;
+}
 
 #endif
