code/Yazi.CFlags.fsti
@@ -5,3 +5,18 @@ val fastest: bool
 
 [@CIfDef]
 val gzip: bool
+
+[@CIfDef]
+val __gnuc__: bool
+
+[@CIfDef]
+val __compcert__: bool
+
+[@CIfDef]
+val _msc_ver: bool
+
+[@CIfDef]
+val _m_arm64: bool
+
+[@CIfDef]
+val _m_x64: bool
