Makefile
@@ -152,7 +152,7 @@ KRML=$(KREMLIN_HOME)/krml
 # easily turn this file into a .h, use -add-include '"Impl_Bignum_Intrinsics.h"'
 # and pass -static-header Impl.Bignum.Intrinsics as described in the
 # documentation.
-HAND_WRITTEN_C_FILES = code/c/Yazi_Allocator.h code/c/Yazi_Z_Stream_Fields.inc code/c/Yazi_CRC32_Z.inc code/c/Yazi_Adler32_Z.inc code/c/Yazi_LZ77_String.inc
+HAND_WRITTEN_C_FILES = code/c/Yazi_Misc.h code/c/Yazi_Z_Stream_Fields.inc code/c/Yazi_CRC32_Z.inc code/c/Yazi_Adler32_Z.inc
 
 # This is now the preferred and recommended way to compile C code with KreMLin.
 #
@@ -182,9 +182,10 @@ dist/Makefile.basic: $(filter-out %prims.krml,$(ALL_KRML_FILES)) $(HAND_WRITTEN_
 	  -warn-error @4@5@18 \
 	  -drop LowStar.ConstBuffer,C.Loops,Spec.*,Prims,Lib.*\
 	  -no-prefix Yazi.Adler32 \
-	  -no-prefix Yazi.CRC32 \
-	  -no-prefix Yazi.Util \
 	  -no-prefix Yazi.CFlags \
+	  -no-prefix Yazi.CRC32 \
+	  -no-prefix Yazi.LZ77 \
+	  -no-prefix Yazi.Util \
 	  -no-prefix Yazi.Types \
 	  -fextern-c \
 	  -ftail-calls \
@@ -195,7 +196,7 @@ dist/Makefile.basic: $(filter-out %prims.krml,$(ALL_KRML_FILES)) $(HAND_WRITTEN_
 	  -bundle Yazi.LZ77=Yazi.LZ77,Yazi.LZ77.*,Yazi.Stream.State \
 	  -add-include '<stdint.h>' \
 	  -add-include '<string.h>' \
-	  -add-early-include '"Yazi_Allocator.h"' \
+	  -add-early-include '"Yazi_Misc.h"' \
 	  -add-include '"kremlin/internal/target.h"' \
 	  -o libz.a
 	sed -i \
